src/Analysis/Instances/Sign/Sign_Exec.thy
@@ -172,9 +172,6 @@ text \<open>The classifier-parametric commutation of the executable and abstract
   declared global needs the executable transfer to commute with the abstract
   transfer at an arbitrary classifier \<open>gs\<close>.\<close>
 
-lemma sign_tf_st_for_reduces: "action_reduces (sign_tf_st_for gs)"
-  by unfold_locales (rule ext, simp)+
-
 theorem sign_tf_st_for_commute:
   "fun_of_resolved_st_q_for gs (sign_tf_st_for gs a s) =
    apply_tf (sign_tf_for gs) a (fun_of_resolved_st_q_for gs s)"
